Partial rewrite

Forward_Hoare.thy
@@ -29,62 +29,16 @@ fun program_to_cterm ctxt p = program_to_term p |> Thm.cterm_of ctxt
 
 section \<open>Invariants\<close>
 
-datatype pc_spec1 = Trivial | Pick int
-type_synonym pc_spec = "pc_spec1 list"
 type_synonym invariant = "mem \<Rightarrow> bool"
 
-fun postcondition1 :: "instruction \<Rightarrow> pc_spec1 \<Rightarrow> invariant \<Rightarrow> invariant option" where
-  "postcondition1 (Set x i) Trivial I = Some (\<lambda>m. m x = i \<and> (\<exists>j. I (m(x:=j))))"
-| "postcondition1 (Guess x) (Pick i) I = Some (\<lambda>m. m x = i \<and> (\<exists>j. I (m(x:=j))))"
-| "postcondition1 (Guess x) Trivial I = Some (\<lambda>m. \<exists>j. I (m(x:=j)))"
-| "postcondition1 (Add x y) Trivial I = (if x\<noteq>y then Some (\<lambda>m. I (m(x:=m x - m y))) else None)"
-| "postcondition1 _ (Pick _) _ = None"
+fun postcondition_trivial :: "instruction \<Rightarrow> invariant \<Rightarrow> invariant" where
+  "postcondition_trivial (Set x i) I = (\<lambda>m. m x = i \<and> (\<exists>j. I (m(x:=j))))"
+| "postcondition_trivial (Guess x) I = (\<lambda>m. \<exists>j. I (m(x:=j)))"
+| "postcondition_trivial (Add x y) I = (\<lambda>m. I (m(x:=m x - m y)))"
 
-fun postcondition :: "program \<Rightarrow> pc_spec \<Rightarrow> invariant \<Rightarrow> invariant option" where
-  "postcondition [] [] I = Some I"
-| "postcondition (c#p) (s#ss) I = (case postcondition1 c s I of Some I' \<Rightarrow> postcondition p ss I' | None \<Rightarrow> None)"
-| "postcondition _ _ _ = None"
-
-lemma pc_length: "postcondition p1 pc1 I \<noteq> None \<Longrightarrow> length p1 = length pc1"
-  apply (induction p1 arbitrary: I pc1)
-  using list.exhaust apply force
-  apply auto
-  apply (case_tac pc1)
-   apply auto
-  by (metis option.case_eq_if option.distinct(1))
-
-
-lemma postcondition': "postcondition (p @ [c]) (ss @ [s]) I =
-  (case postcondition p ss I of Some I' \<Rightarrow> postcondition1 c s I' | None \<Rightarrow> None)"
-proof (cases "length p = length ss")
-  case True
-  then show ?thesis
-  proof (induction arbitrary: I rule:list_induct2)
-    case Nil
-    then show ?case
-      apply (cases "postcondition1 c s I")
-      by auto
-  next
-    case (Cons x xs y ys)
-    show ?case 
-      apply (cases "postcondition1 x y I"; simp)
-      using Cons.IH by blast
-  qed
-next
-  case False
-  then show ?thesis
-    by (metis length_append_singleton nat.inject option.simps(4) pc_length)
-qed
-
-ML \<open>
-datatype pc_spec1 = Trivial | Pick of int
-type pc_spec = pc_spec1 list
-fun pc_spec1_to_term Trivial = \<^const>\<open>Trivial\<close>
-  | pc_spec1_to_term (Pick i) = \<^const>\<open>Pick\<close> $ HOLogic.mk_number HOLogic.intT i
-fun pc_spec_to_term pc = pc |> map pc_spec1_to_term |> HOLogic.mk_list \<^typ>\<open>pc_spec1\<close>
-fun pc_spec_to_cterm ctxt pc = pc_spec_to_term pc |> Thm.cterm_of ctxt
-fun merge_pc pc1 pc2 = SOME (pc1 @ pc2)
-\<close>
+fun postcondition_pick :: "instruction \<Rightarrow> int \<Rightarrow> invariant \<Rightarrow> invariant" where
+  "postcondition_pick (Guess x) i I = (\<lambda>m. m x = i \<and> (\<exists>j. I (m(x:=j))))"
+| "postcondition_pick _ _ _ = undefined"
 
 section \<open>Ranges\<close>
 
@@ -103,18 +57,33 @@ fun merge_ranges (_:program) ((s1,e1):range) ((s2,e2):range) : range option =
 section \<open>Joint stuff\<close>
 
 ML \<open>
-type step_spec = {
+type invariant = {
+  binding: binding,
+  cterm: cterm,
+  const: term
+}
+\<close>
+
+
+ML \<open>
+type hoare = {
   binding: binding,
   range: range,
   program_fragment: program,
   program_fragment_const: term,
-  postcondition: pc_spec,
-  postcondition_ct: cterm,
-  postcondition_const: term,
-  invariant_ct: cterm,
-  invariant_const: term
+  precondition: string,
+  postcondition: string
 }
 \<close>
+
+ML \<open>
+structure Hoare_Data = Proof_Data (
+  type T = { invariants: invariant Symtab.table,
+             hoares: hoare Symtab.table }
+  fun init _ = { invariants=Symtab.empty, hoares=Symtab.empty }
+)
+\<close>
+
 
 ML \<open>
 fun mk_the t = let val oT = fastype_of t in case oT of 
@@ -122,49 +91,42 @@ fun mk_the t = let val oT = fastype_of t in case oT of
  | _ => raise TYPE("mk_the: expected option type",[oT],[t]) end
 \<close>
 
-
 ML \<open>
-structure Steps = Proof_Data (
-  type T = step_spec Symtab.table
-  fun init _ = Symtab.empty
-)
+fun map_invariants f = Hoare_Data.map (fn {invariants,hoares} => {invariants=f invariants, hoares=hoares})
+fun map_hoares f = Hoare_Data.map (fn {invariants,hoares} => {invariants=invariants, hoares=f hoares})
+fun add_invariant0 i = map_invariants (Symtab.update_new (Binding.name_of (#binding i), i))
+fun add_hoare0 i = map_hoares (Symtab.update_new (Binding.name_of (#binding i), i))
+fun get_invariant ctxt name = Symtab.lookup (Hoare_Data.get ctxt |> #invariants) name
+fun get_hoare ctxt name = Symtab.lookup (Hoare_Data.get ctxt |> #hoares) name
 \<close>
 
 ML \<open>
-fun add_spec spec = Steps.map (Symtab.update_new (Binding.name_of (#binding spec), spec))
-fun get_spec name ctxt = Symtab.lookup (Steps.get ctxt) name |> the
+fun add_invariant binding invariant ctxt : invariant * Proof.context = let
+  fun bind suffix = Binding.suffix_name suffix binding
+  val _ = tracing ("Adding invariant "^ Pretty.string_of (Binding.pretty binding) ^ ": " ^ Syntax.string_of_term ctxt (Thm.term_of invariant))
+  val (invariant_const,ctxt) = def' (bind "_inv") invariant ctxt
+  val info : invariant = {binding=binding, const=invariant_const, cterm=invariant}
+  val ctxt = add_invariant0 info ctxt
+  in (info,ctxt) end
 \<close>
 
-
 ML \<open>
-fun make_step binding program range precondition_const postcondition lthy : local_theory = let
+fun add_hoare binding program range (precondition:invariant) (postcondition:invariant) ctxt = let
   fun bind suffix = Binding.suffix_name suffix binding
   val program_fragment = extract_range program range
-  val program_fragment_ct = program_to_cterm lthy program_fragment
-  val _ = tracing ("Program fragment: " ^ Syntax.string_of_term lthy (Thm.term_of program_fragment_ct))
-  val (program_fragment_const,lthy) = 
-      def' (bind "_prog") program_fragment_ct lthy
-  val postcondition_ct = pc_spec_to_cterm lthy postcondition
-  val _ = tracing ("Postcondition: " ^ Syntax.string_of_term lthy (Thm.term_of postcondition_ct))
-  val (postcondition_const,lthy) = def' (bind "_pc") postcondition_ct lthy
-  val invariant_opt_ct = \<^const>\<open>postcondition\<close> 
-        $ program_fragment_const
-        $ postcondition_const
-        $ precondition_const |> Thm.cterm_of lthy
-  val _ = tracing ("Invariant: " ^ Syntax.string_of_term lthy (Thm.term_of invariant_opt_ct))
-  val (invariant_opt_const,lthy) = def' (bind "_inv_opt") invariant_opt_ct lthy
-  val invariant_ct = invariant_opt_const |> mk_the |> Thm.cterm_of lthy
-  val (invariant_const,lthy) = def' (bind "_inv") invariant_ct lthy
-  val spec : step_spec = {binding=binding, range=range, program_fragment=program_fragment, invariant_const=invariant_const,
-    invariant_ct=invariant_ct, postcondition=postcondition, 
-    postcondition_const=postcondition_const, postcondition_ct=postcondition_ct,
-    program_fragment_const=program_fragment_const}
-  val _ = tracing ("Spec: " ^ \<^make_string> spec)
-  val lthy = add_spec spec lthy
-in
-  lthy
-end
+  val program_fragment_ct = program_to_cterm ctxt program_fragment
+  val _ = tracing ("Program fragment: " ^ Syntax.string_of_term ctxt (Thm.term_of program_fragment_ct))
+  val (program_fragment_const,ctxt) = 
+      def' (bind "_prog") program_fragment_ct ctxt
+  val info : hoare = {binding=binding, range=range,
+    precondition=Binding.name_of (#binding precondition),
+    postcondition=Binding.name_of (#binding postcondition),
+    program_fragment=program_fragment, program_fragment_const=program_fragment_const
+  }
+  val ctxt = add_hoare0 info ctxt
+  in (info,ctxt) end
 \<close>
+
 
 definition "pc_imp pc1 pc2 \<longleftrightarrow> (\<forall>m. pc1 m \<longrightarrow> pc2 m)"
 
@@ -175,25 +137,6 @@ section \<open>Experiments\<close>
 ML \<open>
 val test_prog = [Set ("x", 5), Guess "y", Add ("x", "y")] 
 \<close>
-
-definition "start_prog :: program \<equiv> []"
-definition "start_pc :: pc_spec \<equiv> []"
-definition "start_inv :: invariant \<equiv> \<lambda>m::mem. True"
-
-ML \<open>
-val start_spec : step_spec = {
-  binding = \<^binding>\<open>start\<close>,
-  range = (0,0),
-  program_fragment = [],
-  program_fragment_const = \<^term>\<open>start_prog\<close>,
-  postcondition = [],
-  postcondition_ct = \<^cterm>\<open>[]\<close>,
-  postcondition_const = \<^term>\<open>start_pc\<close>,
-  invariant_ct = \<^cterm>\<open>Some (\<lambda>m::mem. True)\<close>,
-  invariant_const = \<^term>\<open>start_inv\<close>
-}
-\<close>
-
 
 ML \<open>
 fun do_cmd source = let
@@ -217,90 +160,78 @@ lemma independent_ofI:
   shows "independent_of B x"
   unfolding independent_of_def using assms by metis
 
-
-lemma newvalue_Guess: 
-  assumes "invariant \<equiv> the invariant_opt"
-  assumes "invariant_opt \<equiv> postcondition prog pc A"
-  assumes "prog \<equiv> [Guess x]"
-  assumes "pc \<equiv> [Pick i]"
+lemma newvalue_Set:
+  assumes "invariant \<equiv> postcondition_trivial (Set x i) A"
   shows "pc_imp invariant (\<lambda>m. m x = i)"
-  unfolding assms(1-4)
+  unfolding assms
   by (rule pc_impI; simp)
 
-lemma newvalue_Set:
-  assumes "invariant \<equiv> the invariant_opt"
-  assumes "invariant_opt \<equiv> postcondition prog pc A"
-  assumes "prog \<equiv> [Set x i]"
-  assumes "pc \<equiv> [Trivial]"
+lemma newvalue_Guess: 
+  assumes "invariant \<equiv> postcondition_pick (Guess x) i A"
   shows "pc_imp invariant (\<lambda>m. m x = i)"
-  unfolding assms(1-4)
+  unfolding assms
   by (rule pc_impI; simp)
 
 lemmas newvalue = newvalue_Set newvalue_Guess
 
-lemma unchanged_Guess: 
-  assumes "invariant \<equiv> the invariant_opt"
-  assumes "invariant_opt \<equiv> postcondition prog pc A"
-  assumes "prog \<equiv> [Guess x]"
-  assumes "pc \<equiv> [s]"
+lemma unchanged_Guess_trivial: 
+  assumes "invariant \<equiv> postcondition_trivial (Guess x) A"
   assumes indep: "independent_of B x"
   assumes imp: "\<And>m. A m \<Longrightarrow> B m"
   shows "pc_imp invariant B"
-  unfolding assms(1-4)
-  apply (cases s; rule pc_impI; simp)
+  unfolding assms(1)
+  apply (rule pc_impI; simp)
+  using indep imp unfolding independent_of_def apply auto
+  by (metis fun_upd_def)+
+
+lemma unchanged_Guess_pick: 
+  assumes "invariant \<equiv> postcondition_pick (Guess x) i A"
+  assumes indep: "independent_of B x"
+  assumes imp: "\<And>m. A m \<Longrightarrow> B m"
+  shows "pc_imp invariant B"
+  unfolding assms(1)
+  apply (rule pc_impI; simp)
   using indep imp unfolding independent_of_def apply auto
   by (metis fun_upd_def)+
 
 lemma unchanged_Add: 
-  assumes "invariant \<equiv> the invariant_opt"
-  assumes "invariant_opt \<equiv> postcondition prog pc A"
-  assumes "prog \<equiv> [Add x y]"
-  assumes "pc \<equiv> [Trivial]"
+  assumes "invariant \<equiv> postcondition_trivial (Add x y) A"
   assumes indep: "independent_of B x"
   assumes xy: "x \<noteq> y"
   assumes imp: "\<And>m. A m \<Longrightarrow> B m"
   shows "pc_imp invariant B"
-  unfolding assms(1-4)
+  unfolding assms
   apply (rule pc_impI)
   using indep imp xy unfolding independent_of_def apply auto
   by (metis fun_upd_def)
 
 lemma unchanged_Set: 
-  assumes "invariant \<equiv> the invariant_opt"
-  assumes "invariant_opt \<equiv> postcondition prog pc A"
-  assumes "prog \<equiv> [Set x i]"
-  assumes "pc \<equiv> [Trivial]"
+  assumes "invariant \<equiv> postcondition_trivial (Set x i) A"
   assumes indep: "independent_of B x"
   assumes imp: "\<And>m. A m \<Longrightarrow> B m"
   shows "pc_imp invariant B"
-  unfolding assms(1-4)
+  unfolding assms(1)
   apply (rule pc_impI)
   using indep imp unfolding independent_of_def apply auto
   by (metis fun_upd_def)
 
-lemmas unchanged = unchanged_Guess unchanged_Add unchanged_Set
+lemmas unchanged = unchanged_Guess_pick unchanged_Guess_trivial unchanged_Add unchanged_Set
 
 lemma wp_Add: 
-  assumes "invariant \<equiv> the invariant_opt"
-  assumes "invariant_opt \<equiv> postcondition prog pc A"
-  assumes "prog \<equiv> [Add x y]"
-  assumes "pc \<equiv> [Trivial]"
+  assumes "invariant \<equiv> postcondition_trivial (Add x y) A"
   assumes distinct: "x \<noteq> y"
   assumes imp: "\<And>m. A m \<Longrightarrow> B (m(x:=m x + m y))"
   shows "pc_imp invariant B"
-  unfolding assms(1-4)
+  unfolding assms(1)
   apply (rule pc_impI)
   using distinct apply simp apply (drule imp)
   by auto
 
 lemma wp_Set:
-  assumes "invariant \<equiv> the invariant_opt"
-  assumes "invariant_opt \<equiv> postcondition prog pc A"
-  assumes "prog \<equiv> [Set x i]"
-  assumes "pc \<equiv> [Trivial]"
+  assumes "invariant \<equiv> postcondition_trivial (Set x i) A"
   assumes imp: "\<And>m. A m \<Longrightarrow> B (m(x:=i))"
   shows "pc_imp invariant B"
-  unfolding assms(1-4)
+  unfolding assms(1)
   apply (rule pc_impI)
   apply simp
   using imp
@@ -309,81 +240,6 @@ lemma wp_Set:
   by auto
 
 lemmas wp = wp_Add wp_Set
-
-lemma valid_Add:
-  fixes inv
-  assumes "inv \<equiv> postcondition prog pc A"
-  assumes "prog \<equiv> [Add x y]"
-  assumes "pc \<equiv> [Trivial]"
-  assumes distinct: "x \<noteq> y"
-  shows "inv \<noteq> None"
-  unfolding assms(1-3) using distinct by simp
-
-
-lemma valid_Set:
-  fixes inv
-  assumes "inv \<equiv> postcondition prog pc A"
-  assumes "prog \<equiv> [Set x i]"
-  assumes "pc \<equiv> [Trivial]"
-  shows "inv \<noteq> None"
-  unfolding assms(1-3) by simp
-
-lemma valid_Guess:
-  fixes inv
-  assumes "inv \<equiv> postcondition prog pc A"
-  assumes "prog \<equiv> [Guess x]"
-  assumes "pc \<equiv> [s]"
-  shows "inv \<noteq> None"
-  unfolding assms(1-3) apply (cases s) by simp_all
-
-lemmas valid = valid_Set valid_Guess valid_Add
-
-ML \<open>
-fun use_facts_tac ctxt thms = 
-  EVERY' (map (fn thm => forward_tac ctxt [thm COMP @{thm pc_impD}]) (rev (tl thms)))
-  THEN' (dresolve_tac ctxt [hd thms COMP @{thm pc_impD}])
-\<close>
-
-(* method use_fact uses fact = frule fact[THEN pc_impD] *)
-
-lemma list_rev_induct2 [consumes 1, case_names Nil snoc]:
-  "length xs = length ys \<Longrightarrow> P [] [] \<Longrightarrow>
-   (\<And>x xs y ys. length xs = length ys \<Longrightarrow> P xs ys \<Longrightarrow> P (xs@[x]) (ys@[y]))
-   \<Longrightarrow> P xs ys"
-  apply (rule list_induct2[where xs="rev xs" and ys="rev ys" and P="\<lambda>xs ys. P (rev xs) (rev ys)", simplified])
-  by auto
-
-lemma pc_merge:
-  assumes "postcondition p1 pc1 I \<noteq> None"
-  shows "postcondition p2 pc2 (the (postcondition p1 pc1 I)) = postcondition (p1 @ p2) (pc1 @ pc2) I"
-  using assms
-proof (cases "length p2 = length pc2")
-  case True
-  then show ?thesis
-  proof (induction rule:list_rev_induct2)
-    case Nil
-    then show ?case
-      using assms by simp
-  next
-    case (snoc p2s p2 pc2s pc2)
-    show ?case
-      unfolding append_assoc[symmetric] postcondition'
-      by (simp add: snoc.IH)
-  qed
-next
-  case False
-  then have 1: "postcondition p2 pc2 I' = None" for I'
-    using pc_length by blast
-  from assms have "length p1 = length pc1"
-    by (rule pc_length)
-  with False have "length (p1@p2) \<noteq> length (pc1@pc2)"
-    by auto
-  then have 2: "postcondition (p1 @ p2) (pc1 @ pc2) I = None"
-    using pc_length by blast
-  from 1 2 
-  show ?thesis
-    by simp
-qed
 
 fun semantics1 :: "instruction \<Rightarrow> mem \<Rightarrow> mem set" where
   "semantics1 (Set x i) m = {m(x:=i)}"
@@ -406,91 +262,62 @@ lemma hoare_cons:
   shows "hoare A (c#p) C"
   using assms unfolding hoare_def apply auto by metis
 
-lemma hoareI1:
-  assumes "postcondition1 c s A = Some C"
-  shows "hoare A [c] C"
-proof (cases c)
-  case (Add x y)
-  show ?thesis
-    unfolding Add
-  proof (cases s)
-    case Trivial
-    show "hoare A [Add x y] C"
-      using assms 
-      unfolding hoare_def Add Trivial
-      apply auto
-      by (smt fun_upd_other fun_upd_same fun_upd_triv fun_upd_upd option.distinct(1) option.inject)
-  next
-    case (Pick i)
-    with assms Add have False
-      by simp
-    then show "hoare A [Add x y] C"
-      by simp
-  qed
-next
-  case (Set x i)
-  show ?thesis
-    unfolding Set
-  proof (cases s)
-    case Trivial
-    show "hoare A [Set x i] C"
-      using assms 
-      unfolding hoare_def Set Trivial
-      apply auto
-      by (metis fun_upd_triv)
-  next
-    case (Pick j)
-    with assms Set have False
-      by simp
-    then show "hoare A [Set x i] C"
-      by simp
-  qed
-next
-  case (Guess x)
-  show ?thesis
-    unfolding Guess
-  proof (cases s)
-    case (Pick j)
-    show "hoare A [Guess x] C"
-      using assms 
-      unfolding hoare_def Guess Pick
-      apply simp
-      by (metis (mono_tags, lifting) fun_upd_idem_iff fun_upd_same fun_upd_upd)
-  next
-    case Trivial
-    show "hoare A [Guess x] C"
-      using assms 
-      unfolding hoare_def Guess Trivial
-      apply simp
-      by (metis fun_upd_triv)
-  qed
-qed
-
-lemma hoareI0:
-  assumes "postcondition p pc A = Some B"
+lemma hoareI:
+  assumes "\<And>m. A m \<Longrightarrow> Bex (semantics p m) B"
   shows "hoare A p B"
-proof -
-  have "length p = length pc"
-    using assms pc_length by auto
-  from this assms show ?thesis
-  proof (induction arbitrary: A rule:list_induct2)
-    case Nil
-    then show ?case by simp
-  next
-    case (Cons c p s pc)
-    then have "postcondition (c # p) (s # pc) A = Some B"
-      by -
-    then obtain C where pc_p: "postcondition p pc C = Some B" and pc_c: "postcondition1 c s A = Some C"
-      apply (cases "postcondition1 c s A")
-      by auto
-    from pc_p have "hoare C p B"
-      using Cons.IH by auto
-    moreover from pc_c have "hoare A [c] C"
-      by (rule hoareI1)
-    ultimately show ?case
-      apply (rule_tac hoare_cons) by auto
-  qed
-qed
+  unfolding hoare_def using assms by simp
+
+lemma valid_Add:
+  assumes "B \<equiv> postcondition_trivial (Add x y) A"
+  assumes "p \<equiv> [Add x y]"
+  assumes distinct: "x \<noteq> y"
+  shows "hoare A p B"
+  apply (rule hoareI)
+  unfolding assms(1-2) using distinct by simp
+
+
+lemma valid_Set:
+  assumes "B \<equiv> postcondition_trivial (Set x i) A"
+  assumes "p \<equiv> [Set x i]"
+  shows "hoare A p B"
+  apply (rule hoareI)
+  unfolding assms
+  apply simp
+  by (metis fun_upd_triv)
+
+lemma valid_Guess_trivial:
+  assumes "B \<equiv> postcondition_trivial (Guess x) A"
+  assumes "p == [Guess x]"
+  shows "hoare A p B"
+  apply (rule hoareI)
+  unfolding assms
+  apply simp
+  by (metis fun_upd_triv)
+
+lemma valid_Guess_pick:
+  assumes "B \<equiv> postcondition_pick (Guess x) i A"
+  assumes "p == [Guess x]"
+  shows "hoare A p B"
+  apply (rule hoareI)
+  unfolding assms
+  apply (rule bexI[of _ "_(x := i)"])
+  apply auto
+  by (metis fun_upd_triv)
+
+lemmas valid = valid_Set valid_Guess_pick valid_Guess_trivial valid_Add
+
+ML \<open>
+fun use_facts_tac ctxt thms = 
+  EVERY' (map (fn thm => forward_tac ctxt [thm COMP @{thm pc_impD}]) (rev (tl thms)))
+  THEN' (dresolve_tac ctxt [hd thms COMP @{thm pc_impD}])
+\<close>
+
+lemma list_rev_induct2 [consumes 1, case_names Nil snoc]:
+  "length xs = length ys \<Longrightarrow> P [] [] \<Longrightarrow>
+   (\<And>x xs y ys. length xs = length ys \<Longrightarrow> P xs ys \<Longrightarrow> P (xs@[x]) (ys@[y]))
+   \<Longrightarrow> P xs ys"
+  apply (rule list_induct2[where xs="rev xs" and ys="rev ys" and P="\<lambda>xs ys. P (rev xs) (rev ys)", simplified])
+  by auto
 
 lemma hoare_conseq:
   assumes "pc_imp A A'"
@@ -499,98 +326,145 @@ lemma hoare_conseq:
   shows "hoare A p B"
   using assms unfolding hoare_def pc_imp_def by blast
 
-lemma hoareI:
-  assumes "B' \<equiv> postcondition p' pc A'"
-  assumes "B' \<noteq> None"
-  assumes AA': "pc_imp A A'"
-  assumes B'B: "pc_imp (the B') B"
-  assumes p'p: "p' = p"
+lemma hoare_conseq':
+  assumes "hoare A' p' B'"
+  assumes "pc_imp A A'"
+  assumes "pc_imp B' B"
+  assumes "p = p'"
   shows "hoare A p B"
-  using AA' B'B apply (rule hoare_conseq)
-  apply (rule hoareI0)
-  using assms(1-2) unfolding p'p by auto
+  using assms unfolding hoare_def pc_imp_def by blast
+
+ML \<open>
+fun hoare_thm ctxt (hoare:string) : cterm = let
+  val hoare = get_hoare ctxt hoare |> the
+  val pre = #precondition hoare |> get_invariant ctxt |> the |> #const
+  val post = #postcondition hoare |> get_invariant ctxt |> the |> #const
+  val prog = #program_fragment_const hoare
+  val prop = \<^const>\<open>hoare\<close> $ pre $ prog $ post |> HOLogic.mk_Trueprop
+  in Thm.cterm_of ctxt prop end
+\<close>
+
+lemma semantics_seq: "semantics (p@q) m = 
+  (\<Union>m'\<in>semantics p m. semantics q m')"
+  sorry
+
+lemma hoare_seq:
+  assumes "hoare A p B"
+  assumes "hoare B q C"
+  shows "hoare A (p@q) C"
+proof (unfold hoare_def, auto)
+  fix m
+  assume "A m"
+  with assms(1) obtain m' where "B m'" and m': "m' \<in> semantics p m"
+    apply atomize_elim unfolding hoare_def by auto
+  with assms(2) obtain m'' where "C m''" and m'': "m'' \<in> semantics q m'"
+    apply atomize_elim unfolding hoare_def by auto
+  from m' m'' have "m'' \<in> semantics (p@q) m"
+    unfolding semantics_seq by auto
+  with \<open>C m''\<close> show "\<exists>m''\<in>semantics (p@q) m. C m''"
+    by auto
+qed
+
+lemma hoare_seq':
+  assumes "hoare A p B"
+  assumes "hoare B q C"
+  assumes "pq = p @ q"
+  shows "hoare A pq C"
+  unfolding assms(3) using assms(1-2) by (rule hoare_seq) 
 
 lemma True
 proof 
 
   define prog where "prog = [Set STR ''x'' 5, Guess STR ''y'', Add STR ''x'' STR ''y'']"
 
-  (* Step 1 *)
+  do \<open>fn ctxt => let
+    val (start_invariant,ctxt) = add_invariant \<^binding>\<open>start\<close> \<^cterm>\<open>(\<lambda>m::mem. True)\<close> ctxt
+    val (hoare,ctxt) = add_hoare \<^binding>\<open>start\<close> test_prog (0,0) start_invariant start_invariant ctxt
+    val _ = \<^print> hoare
+  in ctxt end\<close>
 
-  do \<open>make_step \<^binding>\<open>step1\<close> test_prog (0,1) (#invariant_const start_spec) [Trivial]\<close>
+  (* Step 1: Set x 5 *)
 
-  have step1_exists: "step1_inv_opt \<noteq> None"
-    by (rule valid, fact step1_inv_opt_def, fact step1_prog_def, fact step1_pc_def)
+  do \<open>fn ctxt => let
+    val (post,ctxt) = add_invariant \<^binding>\<open>step1\<close> \<^cterm>\<open>(postcondition_trivial (Set STR ''x'' 5) start_inv)\<close> ctxt
+    val start = get_invariant ctxt "start" |> the
+    val (hoare,ctxt) = add_hoare \<^binding>\<open>step1\<close> test_prog (0,1) start post ctxt 
+    in ctxt end\<close>
+
+  thm step1_inv_def
+
+  ML_val \<open>
+    hoare_thm \<^context> "step1"
+  \<close>
+
+  have step1_valid: "hoare start_inv step1_prog step1_inv"
+    using step1_inv_def step1_prog_def by (rule valid)
 
   have step1_x5: "pc_imp step1_inv (\<lambda>m. m STR ''x'' = 5)"
-    by (rule newvalue, fact step1_inv_def, fact step1_inv_opt_def, fact step1_prog_def, fact step1_pc_def)
+    using step1_inv_def by (rule newvalue)
 
-  (* Step 2 *)
+  (* Step 2: Guess y *)
 
-  do \<open>make_step \<^binding>\<open>step2\<close> test_prog (1,2) (#invariant_const (get_spec "step1" \<^context>)) [Pick ~5]\<close>
+  do \<open>fn ctxt => let
+    val (post,ctxt) = add_invariant \<^binding>\<open>step2\<close>
+       \<^cterm>\<open>postcondition_pick (Guess STR ''y'') (-5) step1_inv\<close> ctxt
+    val pre = get_invariant ctxt "step1" |> the
+    val (hoare,ctxt) = add_hoare \<^binding>\<open>step2\<close> test_prog (1,2) pre post ctxt 
+    in ctxt end\<close>
 
-  have step2_exists: "step2_inv_opt \<noteq> None"
-    by (rule valid, fact step2_inv_opt_def, fact step2_prog_def, fact step2_pc_def)
+  ML_val \<open>hoare_thm \<^context> "step2"\<close>
+  have step2_valid: "hoare step1_inv step2_prog step2_inv"
+    using step2_inv_def step2_prog_def by (rule valid)
 
   have step2_x5: "pc_imp step2_inv (\<lambda>m. m STR ''x'' = 5)"
-    apply (rule unchanged, fact step2_inv_def, fact step2_inv_opt_def, fact step2_prog_def, fact step2_pc_def)
+    using step2_inv_def apply (rule unchanged)
      apply (rule independent_ofI, simp)
     apply (tactic \<open>use_facts_tac \<^context> @{thms step1_x5} 1\<close>)
     by simp
 
   have step2_y5: "pc_imp step2_inv (\<lambda>m. m STR ''y'' = -5)"
-    by (rule newvalue, fact step2_inv_def, fact step2_inv_opt_def, fact step2_prog_def, fact step2_pc_def)
+    using step2_inv_def by (rule newvalue)
 
-  ML_prf \<open>
-    local
-    val ctxt = \<^context>
-    val step1 = get_spec "step1" ctxt
-    val step2 = get_spec "step2" ctxt
-    in
-      val range = merge_ranges test_prog (#range step1) (#range step2) |> the
-      val pc = merge_pc (#postcondition step1) (#postcondition step2) |> the
-    end
-  \<close>
+  have start_step2: "hoare start_inv (step1_prog @ step2_prog) step2_inv"
+    using step1_valid step2_valid by (rule hoare_seq)    
 
-  have start_step2: "step2_inv_opt = postcondition (step1_prog @ step2_prog) (step1_pc @ step2_pc) start_inv"
-    using step1_exists
-    unfolding step2_inv_opt_def step1_inv_def step1_inv_opt_def
-    by (rule pc_merge)
+  (* Step 3: Add x y *)
 
-  (* Step 3 *)
+  do \<open>fn ctxt => let
+    val (post,ctxt) = add_invariant \<^binding>\<open>step3\<close>
+       \<^cterm>\<open>(postcondition_trivial (Add STR ''x'' STR ''y'') step2_inv)\<close> ctxt
+    val pre = get_invariant ctxt "step2" |> the
+    val (hoare,ctxt) = add_hoare \<^binding>\<open>step3\<close> test_prog (2,3) pre post ctxt 
+    in ctxt end\<close>
 
-  do \<open>make_step \<^binding>\<open>step3\<close> test_prog (2,3) (#invariant_const (get_spec "step2" \<^context>)) [Trivial]\<close>
-
-  have step3_exists: "step3_inv_opt \<noteq> None"
-    apply (rule valid, fact step3_inv_opt_def, fact step3_prog_def, fact step3_pc_def)
-    by simp
+  ML_val \<open>hoare_thm \<^context> "step3"\<close>
+  have step3_valid: "hoare step2_inv step3_prog step3_inv"
+    using step3_inv_def step3_prog_def by (rule valid, simp)
 
   have step3_y5: "pc_imp step3_inv (\<lambda>m. m STR ''y'' = -5)"
-    apply (rule unchanged, fact step3_inv_def, fact step3_inv_opt_def, fact step3_prog_def, fact step3_pc_def)
+    using step3_inv_def apply (rule unchanged)
       apply (rule independent_ofI, simp)
      apply simp
     apply (tactic \<open>use_facts_tac \<^context> @{thms step2_y5} 1\<close>)
     by simp
 
   have step3_x0: "pc_imp step3_inv (\<lambda>m. m STR ''x'' = 0)"
-    apply (rule wp_Add, fact step3_inv_def, fact step3_inv_opt_def, fact step3_prog_def, fact step3_pc_def)
+    using step3_inv_def apply (rule wp)
      apply simp
     apply (tactic \<open>use_facts_tac \<^context> @{thms step2_x5 step2_y5} 1\<close>)
     by simp
 
-  have start_step3: "step3_inv_opt \<equiv> postcondition ((step1_prog @ step2_prog) @ step3_prog) ((step1_pc @ step2_pc) @ step3_pc) start_inv"
-    apply (subst pc_merge[symmetric])
-    using start_step2 step2_inv_opt_def step2_pc_def step2_prog_def apply force
-    unfolding step3_inv_opt_def step3_inv_def start_step2[symmetric] step2_inv_def
-    by simp
+  have start_step3: "hoare start_inv prog step3_inv"
+    using start_step2 step3_valid
+    apply (rule hoare_seq')
+    by (simp add: prog_def step1_prog_def step2_prog_def step3_prog_def)
 
   then have "hoare (\<lambda>_. True) prog (\<lambda>m. m STR ''x'' = 0)"
-    apply (rule hoareI)
-       apply (fact step3_exists)
-      apply (force simp: start_inv_def)
-    using step3_x0 step3_inv_def apply simp
-    unfolding step1_prog_def step2_prog_def step3_prog_def prog_def
+    apply (rule hoare_conseq')
+    unfolding start_inv_def apply (simp add: pc_imp_def)
+     apply (rule step3_x0)
     by simp
+
 qed
 
 
